Clean up some Utils functions, missing an eqvt proof

Utils.thy
@@ -1,5 +1,7 @@
 theory Utils imports Syntax begin
 
+(* TODO: Probably just make a lot of these definitions instead of (nominal_) funs. *)
+
 fun slice :: "'a list \<Rightarrow> nat \<Rightarrow> nat \<Rightarrow> 'a list" where
   "slice xs n m = take (m - n) (drop n xs)"
 
@@ -134,7 +136,6 @@ nominal_termination (eqvt)
 lemma env_update_eqvt[eqvt]: "p \<bullet> \<epsilon>[x \<rightarrow> h] = (p \<bullet> \<epsilon>)[p \<bullet> x \<rightarrow> p \<bullet> h]"
   by (induct \<epsilon>) (auto simp add: permute_pure env_update_def)
 
-
 section\<open>Helper for creating formulas\<close>
 
 text\<open>Creates a formula that is the AND of all given subformulas.\<close>
@@ -142,90 +143,58 @@ fun mk_and :: "formula list \<Rightarrow> formula" where
   "mk_and [\<phi>] = \<phi>" |
   "mk_and (\<phi>#\<phi>s) = And \<phi> (mk_and \<phi>s)" |
   "mk_and [] = FTrue"
+lemma mk_and_eqvt[eqvt]: "p \<bullet> mk_and \<phi>s = mk_and (p \<bullet> \<phi>s)"
+  by (induction \<phi>s rule: mk_and.induct) (auto)
 
 text\<open>Predicate for whether an entire instance is equal in the given two heaps.\<close>
-nominal_function mk_instance_eq :: "header_type \<Rightarrow> instanc \<Rightarrow> var \<Rightarrow> var \<Rightarrow> formula" where
+definition mk_instance_eq :: "header_type \<Rightarrow> instanc \<Rightarrow> var \<Rightarrow> var \<Rightarrow> formula" where
   "mk_instance_eq ht i x y = (let hl = header_length ht in
     Eq (Slice (SlInstance x i) 0 hl) (Slice (SlInstance y i) 0 hl))"
-  subgoal by (auto simp add: eqvt_def mk_instance_eq_graph_aux_def Let_def)
-  apply (auto)
-done
-nominal_termination (eqvt)
-  by lexicographic_order
-
-nominal_function foo :: "header_table \<Rightarrow> var \<Rightarrow> var \<Rightarrow> formula" where
-  "foo HT x y = mk_and [mk_instance_eq ht i x y. (i, ht) \<leftarrow> HT]"
-  subgoal apply (auto simp add: eqvt_def foo_graph_aux_def Let_def)
+lemma mk_instance_eq_eqvt[eqvt]:
+  "p \<bullet> mk_instance_eq ht i x y = mk_instance_eq (p \<bullet> ht) (p \<bullet> i) (p \<bullet> x) (p \<bullet> y)"
+  by (auto simp add: mk_instance_eq_def permute_pure Let_def)
 
 text\<open>Instance equality:
 Predicate for whether two heaps are equivalent in terms of all possible instances.
-Corresponds to \<equiv>i in the paper.\<close>
-nominal_function mk_heap_instance_eq :: "header_table \<Rightarrow> var \<Rightarrow> var \<Rightarrow> formula" where
-  "mk_heap_instance_eq ((i,ht)#HT) x y = (let hl = header_length ht in
-   And (Eq (Slice (SlInstance x i) 0 hl) (Slice (SlInstance y i) 0 hl))
-       (mk_heap_instance_eq HT x y))" |
-  "mk_heap_instance_eq [] x y = FTrue"
-  subgoal by (auto simp add: eqvt_def mk_heap_instance_eq_graph_aux_def Let_def)
-  subgoal by (simp)
-  apply (clarify)
-  subgoal for P HT x y by (rule list.exhaust) (auto)
-  apply (auto)
-done
-nominal_termination (eqvt)
-  by lexicographic_order
+Corresponds to \<equiv>_i in the paper.\<close>
+definition mk_heap_eq_instances :: "header_table \<Rightarrow> var \<Rightarrow> var \<Rightarrow> formula" where
+  "mk_heap_eq_instances HT x y = mk_and [mk_instance_eq ht i x y. (i, ht) \<leftarrow> HT]"
+lemma mk_heap_eq_instances_eqvt[eqvt]:
+  "p \<bullet> mk_heap_eq_instances HT x y = mk_heap_eq_instances (p \<bullet> HT) (p \<bullet> x) (p \<bullet> y)"
+  by (auto simp add: mk_heap_eq_instances_def permute_pure)
 
 text\<open>Strict equality:
 Predicate for whether two heaps are equal in all instances and the in/out buffers.
 Corresponds to \<equiv> in the paper.\<close>
-nominal_function mk_heap_eq :: "header_table \<Rightarrow> var \<Rightarrow> var \<Rightarrow> formula" where
+definition mk_heap_eq :: "header_table \<Rightarrow> var \<Rightarrow> var \<Rightarrow> formula" where
   "mk_heap_eq HT x y = And (Eq (Packet x PktIn) (Packet y PktIn))
                     (And (Eq (Packet x PktOut) (Packet y PktOut))
-                    (mk_heap_instance_eq HT x y))"
-  subgoal by (auto simp add: eqvt_def mk_heap_eq_graph_aux_def Let_def)
-  apply (auto)
-done
-nominal_termination (eqvt)
-  by lexicographic_order
+                    (mk_heap_eq_instances HT x y))"
+lemma mk_heap_eq_eqvt[eqvt]: "p \<bullet> mk_heap_eq HT x y = mk_heap_eq (p \<bullet> HT) (p \<bullet> x) (p \<bullet> y)"
+  by (simp add: mk_heap_eq_def permute_pure)
 
-text\<open>Like mk_heap_instance_eq but ignoring the given instance.\<close>
-nominal_function mk_instances_eq_except :: "header_table \<Rightarrow> instanc \<Rightarrow> var \<Rightarrow> var \<Rightarrow> formula" where
-  "mk_instances_eq_except HT i x y = mk_heap_instance_eq [(k,ht)\<leftarrow>HT. k \<noteq> i] x y"
-  subgoal by (auto simp add: eqvt_def mk_instances_eq_except_graph_aux_def Let_def)
-  apply (auto)
-done
-nominal_termination (eqvt)
-  by lexicographic_order
-
-
-nominal_function mk_fields_eq_except_helper :: "field list \<Rightarrow> instanc \<Rightarrow> field_name \<Rightarrow> var \<Rightarrow> var \<Rightarrow> formula"
+text\<open>Like mk_heap_eq_instances but ignoring the given instance.\<close>
+definition mk_heap_eq_instances_except :: "header_table \<Rightarrow> instanc \<Rightarrow> var \<Rightarrow> var \<Rightarrow> formula"
 where
-  "mk_fields_eq_except_helper ((Field f _)#fs) i g x y = (let rem = mk_fields_eq_except_helper fs i g x y in
-    let this = if f = g then FTrue else let (n, m) = field_list_to_range fs f in
-      Eq (Slice (SlInstance x i) n m) (Slice (SlInstance y i) n m) in
-    And this rem)" |
-  "mk_fields_eq_except_helper [] _ _ _ _ = FTrue"
-  subgoal by (auto simp add: eqvt_def mk_fields_eq_except_helper_graph_aux_def)
-  subgoal by (simp)
-  apply (clarify)
-  subgoal for P fs i g x y
-    apply (rule list.exhaust) apply (auto)
-    by (rule field.exhaust) (auto)
-  apply (auto)
-done
-nominal_termination (eqvt)
-  by lexicographic_order
+  "mk_heap_eq_instances_except HT i x y = mk_heap_eq_instances [(k,ht)\<leftarrow>HT. k \<noteq> i] x y"
+lemma mk_heap_eq_instances_except_eqvt[eqvt]:
+  "p \<bullet> mk_heap_eq_instances_except HT i x y = mk_heap_eq_instances_except (p \<bullet> HT) (p \<bullet> i) (p \<bullet> x) (p \<bullet> y)"
+  by (simp add: mk_heap_eq_instances_except_def permute_pure)
 
-text\<open>Predicate for equality of all fields of a specific instance except for one.\<close>
-nominal_function mk_fields_eq_except :: "header_type \<Rightarrow> instanc \<Rightarrow> field_name \<Rightarrow> var \<Rightarrow> var \<Rightarrow> formula"
+definition mk_single_field_eq :: "header_type \<Rightarrow> instanc \<Rightarrow> field_name \<Rightarrow> var \<Rightarrow> var \<Rightarrow> formula"
 where
-  "mk_fields_eq_except (HeaderType _ fs) i g x y = mk_fields_eq_except_helper fs i g x y"
-  subgoal by (auto simp add: eqvt_def mk_fields_eq_except_graph_aux_def)
-  subgoal by (simp)
-  apply (clarify)
-  subgoal for P ht i g x y by (rule header_type.exhaust) (auto)
-  apply (auto)
-done
-nominal_termination (eqvt)
-  by lexicographic_order
+  "mk_single_field_eq ht f i x y = (let (n, m) = header_field_to_range ht f in
+    Eq (Slice (SlInstance x i) n m) (Slice (SlInstance y i) n m))"
+lemma mk_single_field_eq_eqvt[eqvt]:
+  "p \<bullet> mk_single_field_eq ht f i x y = mk_single_field_eq (p \<bullet> ht) (p \<bullet> f) (p \<bullet> i) (p \<bullet> x) (p \<bullet> y)"
+  by (simp add: mk_single_field_eq_def permute_pure)
+
+definition mk_fields_eq_except :: "header_type \<Rightarrow> instanc \<Rightarrow> field_name \<Rightarrow> var \<Rightarrow> var \<Rightarrow> formula"
+where
+  "mk_fields_eq_except ht i g x y = (case ht of HeaderType _ fs \<Rightarrow>
+    mk_and [mk_single_field_eq ht f i x y. (Field f _) \<leftarrow> fs, f \<noteq> g])"
+lemma mk_fields_eq_except_eqvt[eqvt]:
+  "p \<bullet> mk_fields_eq_except ht i g x y = mk_fields_eq_except (p \<bullet> ht) (p \<bullet> i) (p \<bullet> g) (p \<bullet> x) (p \<bullet> y)"
+  sorry
 
 end
